theories/tree_borrows/examples/delete_read_unprotected.v
@@ -114,7 +114,7 @@ Proof.
   source_pures. source_bind (Copy _).
   iApply (source_copy_any with "Htag_i Hi_s"). 1: done.
   2: simpl; lia. 1: rewrite read_range_heaplet_to_list // Z.sub_diag /= //.
-  iIntros (v_res) "Hi_s Htag_i %Hv_res_maybepoison". source_pures. source_finish.
+  iIntros (v_res) "Hi_s Htag_i Hv_res_maybepoison". source_pures. source_finish.
   sim_pures.
 
 
@@ -123,7 +123,7 @@ Proof.
   sim_pures.
   sim_val. iModIntro. iSplit; first done.
   (* prove that the values are in simulation (by case-analyzing what was poison when) *)
-  destruct Hv_res_maybepoison as [->| ->]; (iSplit; last done).
+  iDestruct "Hv_res_maybepoison" as "[->| (%id&(%Hp1&->)&Hpp)]"; (iSplit; last done).
   - done.
   - done.
 Qed.
