theories/tree_borrows/trees_equal/disabled_tag_rejects_read_precisely.v
@@ -1,0 +1,183 @@
+From iris.proofmode Require Export proofmode.
+From iris.bi.lib Require Import fractional.
+From iris.base_logic.lib Require Import ghost_map.
+From simuliris.base_logic Require Export gen_sim_prog.
+From simuliris.simulation Require Export slsls gen_log_rel.
+From simuliris.simulation Require Import lifting.
+From simuliris.tree_borrows Require Import tkmap_view.
+From simuliris.tree_borrows Require Export defs.
+From simuliris.tree_borrows Require Export steps_wf.
+From simuliris.tree_borrows Require Import steps_progress.
+From simuliris.tree_borrows.trees_equal Require Import disabled_in_practice random_lemmas.
+From iris.prelude Require Import options.
+
+Section disabled_tag_rejects_reads_precisely.
+
+  Context (C : call_id_set).
+
+
+
+  Lemma pseudo_disabled_no_child_access tr acc tg_acc it_wit l b range lp :
+    wf_tree tr →
+    range'_contains range l →
+    ParentChildIn (itag it_wit) tg_acc tr →
+    tree_lookup tr (itag it_wit) it_wit →
+    item_lookup it_wit l = mkPerm PermLazy lp →
+    pseudo_disabled C tr (itag it_wit) l lp (iprot it_wit) →
+    memory_access_maybe_nonchildren_only b acc C tg_acc range tr = None.
+  Proof.
+    intros Hwf Hrange HPCI Hlookup Hitlookup Hdis.
+    inversion Hdis as [px Hreallydis Hpx|tg_cs it_cs lpx prx Hrelcs Hlucs Hprotcs Hitlucs HIMcs]; simplify_eq.
+    - destruct (memory_access_maybe_nonchildren_only b acc C tg_acc range tr) as [tr'|] eqn: Hc; last done.
+      exfalso. eapply apply_access_spec_per_node in Hc as (it'&Hit'&Hitlookup2).
+      2-3: apply Hlookup.
+      eapply eq_sym, mk_is_Some in Hit'.
+      rewrite /rel_dec decide_True // in Hit'.
+      rewrite /item_apply_access in Hit'.
+      setoid_rewrite is_Some_ignore_bind in Hit'.
+      setoid_rewrite <- mem_apply_range'_success_condition in Hit'.
+      specialize (Hit' _ Hrange).
+      erewrite maybe_non_children_only_no_effect in Hit'. 2: by intros ??.
+      rewrite /item_lookup in Hitlookup.
+      rewrite Hitlookup in Hit'. destruct acc; rewrite /apply_access_perm /apply_access_perm_inner /= in Hit'; by destruct Hit'.
+    - destruct (memory_access_maybe_nonchildren_only b acc C tg_acc range tr) as [tr'|] eqn: Hc; last done.
+      exfalso. eapply apply_access_spec_per_node in Hc as (it'&Hit'&Hitlookup2).
+      2-3: apply Hlucs.
+      eapply eq_sym, mk_is_Some in Hit'.
+      enough (rel_dec tr tg_acc (itag it_cs) = Foreign Cousin) as Hfgn.
+      { rewrite Hfgn in Hit'.
+        rewrite /item_apply_access in Hit'.
+        setoid_rewrite is_Some_ignore_bind in Hit'.
+        setoid_rewrite <- mem_apply_range'_success_condition in Hit'.
+        specialize (Hit' _ Hrange).
+        erewrite maybe_non_children_only_no_effect in Hit'. 2: by intros ??.
+        rewrite bool_decide_eq_true_2 // in Hit'.
+        rewrite /item_lookup in Hitlucs.
+        rewrite Hitlucs in Hit'. destruct acc; rewrite /apply_access_perm /apply_access_perm_inner /= in Hit'; by destruct Hit'. }
+      eapply tree_lookup_correct_tag in Hlucs as Htg; subst tg_cs.
+      rewrite /rel_dec. rewrite decide_False.
+      2: { intros HPCI2. eapply cousins_have_disjoint_children. 4: exact Hrelcs. 4: exact HPCI. 4: done.
+           all: eapply Hwf. 2: apply Hlookup. 2: apply Hlucs. eapply contains_child; first exact HPCI. apply Hlookup. }
+      rewrite decide_False //.
+      intros HPCI2.
+      rewrite /rel_dec in Hrelcs.
+      destruct decide as [Hd1|Hd2] in Hrelcs; try done.
+      rewrite decide_True // in Hrelcs.
+      eapply ParentChild_transitive. 1: exact HPCI. done.
+  Qed.
+
+  Lemma is_disabled_no_child_access tr acc tg_acc tg_wit it_wit l b range :
+    wf_tree tr →
+    range'_contains range l →
+    ParentChildIn tg_wit tg_acc tr →
+    tree_lookup tr tg_wit it_wit →
+    is_disabled C tr tg_wit l (item_lookup it_wit l) (iprot it_wit) →
+    memory_access_maybe_nonchildren_only b acc C tg_acc range tr = None.
+  Proof.
+    intros Hwf Hrange HPCI Hlookup Hdis.
+    eapply tree_lookup_correct_tag in Hlookup as Htg; subst tg_wit.
+    inversion Hdis as [px Hreallydis Hpx|lp prot Hpseudo Hlookup2 Hpx].
+    - destruct (memory_access_maybe_nonchildren_only b acc C tg_acc range tr) as [tr'|] eqn: Hc; last done.
+      exfalso. eapply apply_access_spec_per_node in Hc as (it'&Hit'&Hitlookup).
+      2-3: apply Hlookup.
+      eapply eq_sym, mk_is_Some in Hit'.
+      rewrite /rel_dec decide_True // in Hit'.
+      rewrite /item_apply_access in Hit'.
+      setoid_rewrite is_Some_ignore_bind in Hit'.
+      setoid_rewrite <- mem_apply_range'_success_condition in Hit'.
+      specialize (Hit' _ Hrange).
+      erewrite maybe_non_children_only_no_effect in Hit'. 2: by intros ??.
+      rewrite /item_lookup in Hreallydis.
+      rewrite -Hreallydis in Hit'. destruct acc; rewrite /apply_access_perm /apply_access_perm_inner /= in Hit'; by destruct Hit'.
+    - eapply pseudo_disabled_no_child_access. 6: done. all: done.
+  Qed.
+
+  Lemma disabled_in_practice_no_access tr acc tg_wit tg l b range :
+    wf_tree tr →
+    range'_contains range l →
+    disabled_in_practice C tr tg tg_wit l →
+    memory_access_maybe_nonchildren_only b acc C tg range tr = None.
+  Proof.
+    intros Hwf Hrange Hdis.
+    induction Hdis as [it_witness incl H1 H2 H3].
+    eapply is_disabled_no_child_access. 1: done. 1: exact Hrange. 3: done. 2: done.
+    rewrite /rel_dec in H1. destruct decide; done.
+  Qed.
+
+  Lemma disabled_tag_no_access b tr acc tg l range :
+    wf_tree tr →
+    disabled_tag_at C tr tg l →
+    range'_contains range l →
+    memory_access_maybe_nonchildren_only b acc C tg range tr = None.
+  Proof.
+    intros Hwf (wit&Hwit) Hrange.
+    by eapply disabled_in_practice_no_access.
+  Qed.
+
+  Lemma read_fails_disabled_tag_or_prot_act_child b tg ittg range tr :
+    wf_tree tr →
+    protected_parents_not_disabled C tr →
+    no_active_cousins C tr →
+    tree_lookup tr tg ittg →
+    (* ReservedIM can be temporarily disabled, we can not handle this *)
+    (∀ l, range'_contains range l → perm (item_lookup ittg l) ≠ ReservedIM) →
+    memory_access_maybe_nonchildren_only b AccessRead C tg range tr = None →
+    ∃ l, range'_contains range l ∧ (disabled_tag_at C tr tg l ∨
+         (* we never have things that have active children, so this case will be contradictory *)
+         (active_child C tr tg l ∧ b = false)).
+  Proof.
+    intros Hwf Hndis Hnac Hittg HNoIM HNone.
+    eapply apply_access_fail_condition in HNone.
+    eapply exists_node_eqv_existential in HNone as (it&Hexit&HNone).
+    eapply exists_node_to_tree_lookup in Hexit as Hit. 2: apply Hwf.
+    rewrite /item_apply_access in HNone.
+    rewrite /permissions_apply_range' in HNone.
+    eapply bind_None in HNone as [HNone|(x&Hx&HHx)]. 2: done.
+    eapply mem_apply_range'_fail_condition in HNone as (l&Hl&Hll).
+    specialize (Hndis (itag it)). setoid_rewrite every_child_ParentChildIn in Hndis. 2: eapply Hwf.
+    2: eapply Hwf, Hit.
+    ospecialize (Hndis it _ (itag it) _ _). 1: apply Hit. 2: left; done. 1: eapply Hwf, Hit.
+    eapply every_node_iff_every_lookup in Hndis. 2: { intros x Hx%Hwf. by eapply unique_lookup. }
+    2: apply Hit. specialize (Hndis eq_refl l).
+    exists l. split; first done.
+    destruct (rel_dec tr tg (itag it)) as [[ii|]|] eqn:Hreldec.
+    - destruct b; first done.
+      change (default _ _) with (item_lookup it l) in Hll.
+      right. split; last done. exists it, ii.
+      destruct (item_lookup it l) as [ini pp]. simpl in *.
+      split; first done.
+      rewrite rel_dec_flip2 Hreldec /=. split; first done.
+      rewrite /= in Hll.
+      destruct ini, pp as [[]| | | |], (bool_decide (protector_is_active (iprot it) C)) eqn:Hbd; simpl in *; try done.
+      2: { exfalso. ospecialize (Hndis eq_refl _ eq_refl); last done. by eapply bool_decide_eq_true_1. }
+      split; first done.
+      eapply bool_decide_eq_true_1; done.
+    - rewrite maybe_non_children_only_no_effect in Hll. 2: done.
+      change (default _ _) with (item_lookup it l) in Hll.
+      left. exists tg. econstructor. 1: by rewrite rel_dec_refl.
+      1: exact Hittg.
+      ospecialize (Hnac _ _ _ _ l Hittg Hit Hreldec).
+      rewrite bool_decide_decide in Hll. destruct (item_lookup it l) as [[] [[]| | | |]] eqn:Heqitl, (decide (protector_is_active (iprot it) C)) as [Hp|].
+      all: simpl in Hll; try discriminate Hll.
+      2: by specialize (Hndis eq_refl Hp eq_refl).
+      destruct (item_lookup ittg l) as [ini prm] eqn:Heq.
+      destruct ini.
+      { destruct prm as [[]| | | |].
+        6: econstructor.
+        all: (ospecialize (Hnac _ eq_refl); last done).
+        1,2,5: right; rewrite Heq; split; last done; simpl; eauto.
+        2: left; rewrite Heq; done.
+        exfalso. specialize (HNoIM l Hl). rewrite Heq in HNoIM. done. }
+      econstructor.
+      econstructor. 1: exact Hreldec. 1: done. 1: done. 1: done.
+      intros ->. specialize (HNoIM l Hl). rewrite Heq in HNoIM. done.
+    - left. exists (itag it). econstructor. 1: exact Hreldec. 1: done.
+      rewrite maybe_non_children_only_no_effect in Hll. 2: done.
+      change (default _ _) with (item_lookup it l) in Hll.
+      destruct (item_lookup it l) as [ini [[]| | | |]] eqn:Heqitl.
+      1-5: rewrite /apply_access_perm /apply_access_perm_inner /= most_init_comm /= Tauto.if_same /= // in Hll.
+      destruct ini. 1: econstructor 1.
+      econstructor 2. econstructor 1.
+  Qed.
+
+End disabled_tag_rejects_reads_precisely.
